added prettified version of Univ-lemma

theories/TM/Hyperlinked.v
@@ -1,10 +1,11 @@
 From Undecidability Require Import TM.Prelim.
 From Undecidability Require Import TM.TM.
-From Undecidability.TM Require Import Basic.Mono Basic.Null Compound.Multi.
+From Undecidability Require Import TM.Code.ProgrammingTools.
+
 
 (** This file is meant as an entry point for the hyperlinks in the paper. For [Check]s, just click them to get to the lemma. *)
 
-
+From Undecidability.TM Require Import Basic.Mono Basic.Null Compound.Multi.
 Section PrimitiveMachines.
 
   Check Mono.ReadChar_Sem.
@@ -17,3 +18,105 @@ Section PrimitiveMachines.
 
 End PrimitiveMachines.
 
+
+From Undecidability.TM Require Import Univ.StepTM PrettyBounds.UnivBounds PrettyBounds.UnivSpaceBounds.
+From Undecidability Require Import Univ.LookupAssociativeListTM.
+From Undecidability Require Import Basic.Duo.
+From Undecidability Require Import Code.CaseFin Code.CaseList Code.CasePair.
+From Undecidability Require Import Univ.LookupAssociativeListTM.
+
+Require Import PslBase.Bijection. (* [injective] *)
+
+Section UniversalMachine.
+
+
+  Variable (sigM : finType).
+
+  Notation sigGraph := (sigList (sigPair (sigPair (option sigM) sigState) (sigPair (option sigM * move) sigState))).
+
+  (** The alphabet of [Univ] *)
+  Variable (sig : finType).
+  Variable (retr_sigGraph_sig : Retract sigGraph sig).
+  Variable (retr_sigTape_sig : Retract sigM sig).
+
+  (** Encoding of the current state number *)
+  Local Definition retr_sigCurrentStateNumber_sigGraph : Retract sigNat sigGraph :=
+    Retract_sigList_X (Retract_sigPair_X _ (Retract_sigPair_Y _ (Retract_sigPair_Y _ _))).
+  Local Definition retr_sigCurrentStateNumber_sig : Retract sigNat sig :=
+    ComposeRetract retr_sigGraph_sig retr_sigCurrentStateNumber_sigGraph.
+
+  (** Encoding of the current state (= halt bit + number) *)
+  Local Definition retr_sigCurrentState_sigGraph : Retract sigState sigGraph :=
+    Retract_sigList_X (Retract_sigPair_X _ (Retract_sigPair_Y _ (Retract_id _))).
+  Local Definition retr_sigCurrentState_sig : Retract sigState sig := ComposeRetract retr_sigGraph_sig retr_sigCurrentState_sigGraph.
+
+  (** Encoding of final bit of the current state *)
+  Local Definition retr_sigCurrentStateFinal_sigGraph : Retract bool sigGraph :=
+    Retract_sigList_X (Retract_sigPair_X _ (Retract_sigPair_Y _ (Retract_sigPair_X _ _))).
+  Local Definition retr_sigCurrentStateFinal_sig : Retract bool sig := ComposeRetract retr_sigGraph_sig retr_sigCurrentStateFinal_sigGraph.
+
+  (** Encoding of the next state *)
+  Local Definition retr_sigNextState_sigGraph : Retract sigState sigGraph := Retract_sigList_X (Retract_sigPair_Y _ _).
+  Local Definition retr_sigNextState_sig : Retract sigState sig := ComposeRetract retr_sigGraph_sig retr_sigNextState_sigGraph.
+
+  (** Encoding the current symbol *)
+  Local Definition retr_sigCurrentSymbol_sigGraph : Retract (option sigM) sigGraph := Retract_sigList_X (Retract_sigPair_X _ (Retract_sigPair_X _ _)).
+  Local Definition retr_sigCurrentSymbol_sig: Retract (option sigM) sig := ComposeRetract retr_sigGraph_sig retr_sigCurrentSymbol_sigGraph.
+
+  (** Encoding of actions *)
+  Local Definition retr_act_sigGraph : Retract (option sigM * move) sigGraph := _.
+  Local Definition retr_act_sig : Retract (option sigM * move) sig := ComposeRetract retr_sigGraph_sig retr_act_sigGraph.
+
+  (** Encoding of the keys for [Lookup] ([option sig * Q]) *)
+  Local Definition retr_key_sigGraph : Retract _ sigGraph := Retract_sigList_X (Retract_sigPair_X _ (Retract_id _)).
+  Local Definition retr_key_sig : Retract _ sig := ComposeRetract retr_sigGraph_sig retr_key_sigGraph.
+
+  (** Encoding of the value for [Lookup] ([option sig * Q]) *)
+  Local Definition retr_value_sigGraph : Retract _ sigGraph := Retract_sigList_X (Retract_sigPair_Y _ (Retract_id _)).
+  Local Definition retr_value_sig : Retract _ sig := ComposeRetract retr_sigGraph_sig retr_value_sigGraph.
+
+  
+  Local Instance Encode_graph : codable sigGraph (list ((option sigM * (bool * nat)) * ((option sigM * move) * (bool * nat)))) :=
+    (Encode_list
+       (Encode_pair (Encode_pair (Encode_Finite _) (Encode_pair Encode_bool Encode_nat))
+                    (Encode_pair (Encode_Finite _) (Encode_pair Encode_bool Encode_nat)))).
+
+  Definition Univ_T_pretty : tRel sig^+ 6 :=
+    fun tin k =>
+      exists (M : mTM sigM 1),
+        let c := proj1_sig (Univ_nice.Univ_steps_nice M) in
+        exists (tp : tape sigM) (q : states M) (k' : nat) (q' : states M) (tp' : tape sigM),
+        tin[@Fin0] = mapTape (fun s => inr (Retr_f (Retract := retr_sigTape_sig) s)) tp /\
+        tin[@Fin1] ≃(retr_sigGraph_sig) (graph_of_TM M) /\
+        tin[@Fin2] ≃(retr_sigCurrentState_sig) (halt q, index q) /\
+        isRight tin[@Fin3] /\ isRight tin[@Fin4] /\ isRight tin[@Fin5] /\
+        loopM (mk_mconfig q [|tp|]) k' = Some (mk_mconfig q' [|tp'|]) /\
+        c* (size k' * size (graph_of_TM M)) <= k.
+
+
+  (** This lemma ransforms the lemma we proofed in Coq to the more readable version in the paper. *)
+  Lemma Univ_Terminates_pretty : projT1 (Univ _ _) ↓ Univ_T_pretty.
+  Proof.
+    eapply TerminatesIn_monotone.
+    {apply Univ_Terminates. }
+    unfold Univ_T_pretty,Univ_T.
+    unfold containsWorkingTape,containsTrans,containsState.
+    intros tin k.
+    apply Morphisms_Prop.ex_impl_morphism;intro M;hnf.
+    apply Morphisms_Prop.ex_impl_morphism;intro tp;hnf.
+    apply Morphisms_Prop.ex_impl_morphism;intro q;hnf.
+    apply Morphisms_Prop.ex_impl_morphism;intro k';hnf.
+    apply Morphisms_Prop.ex_impl_morphism;intro q';hnf.
+    apply Morphisms_Prop.ex_impl_morphism;intro tp';hnf.
+
+    intros (?&?&?&?&?&?&?&Heq).
+    repeat eapply conj.
+    1-3,5:easy.
+    -intros i. destruct_fin i. all:easy.
+    -assert (Heq':=proj2_sig (Univ_nice.Univ_steps_nice M)).
+     unfold PrettyBounds.dominatedWith in Heq'.
+     rewrite Heq'.
+     rewrite <- Heq. reflexivity.
+  Qed.
+
+End UniversalMachine.
